PAC_Checker2/EPAC_Perfectly_Shared_Vars.thy
@@ -1,629 +1,140 @@
 theory EPAC_Perfectly_Shared_Vars
-  imports EPAC_Checker_Specification
-    PAC_Checker.PAC_Checker (*for vars_llist*)
-    EPAC_Checker (*for vars_llist*)
+  imports EPAC_Perfectly_Shared
+    PAC_Checker.PAC_Checker_Relation
+    PAC_Checker.PAC_Map_Rel
 begin
+thm import_variableS_def
+  term hm.assn
+  term iam.assn
+  term is_iam
+  term iam_rel
 
-text \<open>We now introduce sharing of variables to make a more efficient representation possible.\<close>
+type_synonym ('string2, 'nat) shared_vars_c = \<open>'string2 list \<times> ('string2, 'nat) fmap\<close>
 
-section \<open>Perfectly sharing of elements\<close>
+definition perfect_shared_vars_rel_c :: \<open>('string2 \<times> 'string) set \<Rightarrow> (('string2, nat) shared_vars_c \<times> (nat, 'string)shared_vars) set\<close> where
+  \<open>perfect_shared_vars_rel_c R =
+  {((\<V>, \<A>), (\<D>', \<V>', \<A>')). (\<forall>i\<in>#dom_m \<V>'. i < length \<V>) \<and>
+  (\<forall>i\<in>#dom_m \<V>'. i < length \<V> \<and> (\<V> ! i, the (fmlookup \<V>' i))\<in> R) \<and>
+  (\<A>, \<A>') \<in> \<langle>R,nat_rel\<rangle>fmap_rel}\<close>
 
-subsection \<open>Definition\<close>
-  
-type_synonym ('nat, 'string) shared_vars = \<open>'string multiset \<times> ('nat, 'string) fmap \<times> ('string, 'nat) fmap\<close>
+text \<open>Random conditions with the idea to use machine words eventually\<close>
 
-definition perfectly_shared_vars
-  :: \<open>'string multiset \<Rightarrow>  ('nat, 'string) shared_vars \<Rightarrow> bool\<close>
-where
-  \<open>perfectly_shared_vars \<V> = (\<lambda>(\<D>, V, V').
-  set_mset (dom_m V') = set_mset \<V> \<and> \<D> = \<V> \<and> 
-  (\<forall>i \<in>#dom_m V. fmlookup V' (the (fmlookup V i)) = Some i) \<and>
-  (\<forall>str \<in>#dom_m V'. fmlookup V (the (fmlookup V' str)) = Some str) \<and>
-  (\<forall>i j. i\<in>#dom_m V \<longrightarrow> j\<in>#dom_m V \<longrightarrow> (fmlookup V i = fmlookup V j \<longleftrightarrow> i = j)))\<close>
+definition find_new_idx_c :: \<open>('string, nat) shared_vars_c \<Rightarrow> (memory_allocation \<times> nat)  nres\<close> where
+  \<open>find_new_idx_c = (\<lambda>(\<V>, \<A>). let k = length \<V> in if k < 2^63-1 then RETURN (Allocated, k) else RETURN (Mem_Out, 0) )\<close>
 
-abbreviation fmlookup_direct :: \<open>('a, 'b) fmap \<Rightarrow> 'a \<Rightarrow> 'b\<close> (infix "\<propto>" 70) where
-  \<open>fmlookup_direct A b \<equiv> the (fmlookup A b)\<close>
+definition import_variable_c :: \<open>'string \<Rightarrow>  ('string, nat) shared_vars_c \<Rightarrow> (memory_allocation \<times> ('string, nat) shared_vars_c \<times> nat)  nres\<close> where
+  \<open>import_variable_c v = (\<lambda>(\<V>, \<A>). do {
+  (err, k') \<leftarrow> find_new_idx_c (\<V>, \<A>);
+  if alloc_failed err then do {let k'=k'; RETURN (err, (\<V>, \<A>), k')}
+  else do{
+    ASSERT(k' < 2^63-1);
+    RETURN (Allocated, (\<V> @ [v], fmupd v k' \<A>), k')
+    }
+  })\<close>
 
-lemma perfectly_shared_vars_simps:
-  assumes \<open>perfectly_shared_vars \<V> (VV')\<close>
-  shows \<open>str \<in># \<V> \<longleftrightarrow> str \<in># dom_m (snd (snd VV'))\<close>
-  using assms
-  unfolding perfectly_shared_vars_def
-  apply auto
-  done
 
-lemma perfectly_shared_add_new_var:
-  fixes V :: \<open>('nat, 'string) fmap\<close> and
-    v :: \<open>'string\<close>
-  assumes \<open>perfectly_shared_vars \<V> (D, V, V')\<close> and
-    \<open>v \<notin># \<V>\<close> and
-    k_notin[simp]: \<open>k \<notin># dom_m V\<close>
-  shows \<open>perfectly_shared_vars (add_mset v \<V>) (add_mset v D, fmupd k v V, fmupd v k V')\<close>
+lemma import_variable_c_import_variableS:
+  fixes A' :: \<open>(nat,'string) shared_vars\<close>
+  assumes
+    A: \<open>(A,A')\<in>perfect_shared_vars_rel_c R\<close> and
+    v: \<open>(v,v')\<in>R\<close> \<open>single_valued R\<close> \<open>single_valued (R\<inverse>)\<close>
+  shows \<open>import_variable_c v A \<le>\<Down>(Id \<times>\<^sub>r (perfect_shared_vars_rel_c R \<times>\<^sub>r nat_rel)) (import_variableS v' A')\<close>
 proof -
-  have
-    DV[simp]: \<open>D = \<V>\<close> and
-    V'\<V>: \<open>set_mset (dom_m V') = set_mset \<V>\<close> and
-    map: \<open>\<And>i. i \<in>#dom_m V \<Longrightarrow> fmlookup V' (the (fmlookup V i)) = Some i\<close> and
-    map_str: \<open>\<And>str. str \<in>#dom_m V' \<Longrightarrow> fmlookup V (the (fmlookup V' str)) = Some str\<close> and
-    perfect: \<open>\<And>i j.  i\<in>#dom_m V \<Longrightarrow> j\<in>#dom_m V \<Longrightarrow> fmlookup V i = fmlookup V j \<longleftrightarrow> i = j\<close>
-    using assms unfolding perfectly_shared_vars_def
+  have [refine]: \<open>RETURN x2g \<le> \<Down> Id (RES UNIV)\<close> for x2g :: nat
     by auto
-  have v_notin[simp]: \<open>v \<notin># dom_m V'\<close>
-    using V'\<V> assms(2) by blast
-  show ?thesis
-    unfolding perfectly_shared_vars_def prod.simps
-  proof (intro conjI allI ballI impI)
-    show \<open>add_mset v D = add_mset v \<V>\<close>
-      using DV by auto
-    show \<open>set_mset (dom_m (fmupd v k V')) = set_mset (add_mset v \<V>)\<close>
-      using V'\<V> in_remove1_mset_neq by fastforce
- 
-    show \<open>fmlookup (fmupd v k V') (fmupd k v V \<propto> i) = Some i\<close>
-      if \<open>i \<in># dom_m (fmupd k v V)\<close>
-      for i
-      using map[of i] that v_notin
-      by (auto dest!: indom_mI simp del: v_notin)
+  have [refine]: \<open>find_new_idx_c a \<le> \<Down> {((err, k), (err', k')). err=err' \<and> k=k' \<and> (\<not>alloc_failed err \<longrightarrow> k < 2^63-1 \<and> k = length (fst a))} (find_new_idx b)\<close>
+    if \<open>(a,b) \<in> perfect_shared_vars_rel_c R\<close>
+    for b :: \<open>(nat,'string) shared_vars\<close> and a
+    using that unfolding find_new_idx_c_def find_new_idx_def
+    by (cases b; cases a)
+      (auto intro!: RETURN_RES_refine simp: Let_def perfect_shared_vars_rel_c_def)
 
-    show \<open>fmlookup (fmupd k v V) (fmupd v k V' \<propto> str) = Some str\<close>
-      if \<open>str \<in># dom_m (fmupd v k V')\<close>
-      for str
-      using map_str[of str] that k_notin
-      by (auto dest!: indom_mI simp del: k_notin)
-    show \<open>(fmlookup (fmupd k v V) i = fmlookup (fmupd k v V) j) = (i = j)\<close>
-      if \<open>i \<in># dom_m (fmupd k v V)\<close> and
-        \<open>j \<in># dom_m (fmupd k v V)\<close>
-      for i j
-      using perfect[of i j] that
-      using indom_mI[of V i] map[of i] indom_mI[of V j] map[of j] indom_mI[of V' v]
-      apply (auto simp: eq_commute[of \<open>Some _\<close> \<open>fmlookup V _\<close>])
-      apply auto
-      done
-  qed
+  show ?thesis
+    unfolding import_variable_c_def import_variableS_def find_new_idx_def[symmetric]
+    apply refine_vcg
+    subgoal using A by (auto simp: perfect_shared_vars_rel_c_def)
+    subgoal by auto
+    subgoal using A by (auto simp: perfect_shared_vars_rel_c_def)
+    subgoal by auto
+    subgoal
+      using A v by (force simp: perfect_shared_vars_rel_c_def dest: in_diffD intro!: fmap_rel_fmupd_fmap_rel)
+   done
 qed
 
-lemma perfectly_shared_vars_remove_update:
-  assumes \<open>perfectly_shared_vars (add_mset v \<V>) (D, V, V')\<close> and
-    \<open>v \<notin># \<V>\<close>
-  shows \<open>perfectly_shared_vars  \<V> (remove1_mset v D, fmdrop (V' \<propto> v) V, fmdrop v V')\<close>
-  using assms
-  unfolding perfectly_shared_vars_def
-  by (fastforce simp: distinct_mset_dom distinct_mset_remove1_All)
 
-
-section \<open>Refinement\<close>
-
-datatype memory_allocation =
-  Allocated | alloc_failed: Mem_Out
-
-type_synonym ('nat, 'string) vars = \<open>'string multiset\<close>
-
-definition perfectly_shared_var_rel :: \<open>('nat,'string) shared_vars \<Rightarrow> ('nat \<times> 'string) set\<close> where
-  \<open>perfectly_shared_var_rel = (\<lambda>(\<D>, \<V>, \<V>'). br (\<lambda>i. \<V> \<propto> i) (\<lambda>i. i \<in># dom_m \<V>))\<close>
-
-definition perfectly_shared_vars_rel :: \<open>(('nat,'string) shared_vars \<times> ('nat, 'string) vars) set\<close>
-where
-  \<open>perfectly_shared_vars_rel = {(\<A>, \<V>). perfectly_shared_vars \<V> \<A>}\<close>
-
-definition import_variableS
-  :: \<open>'string \<Rightarrow> ('nat, 'string) shared_vars \<Rightarrow>
-  (memory_allocation \<times> ('nat, 'string) shared_vars \<times> 'nat) nres\<close>
-where
-  \<open>import_variableS v = (\<lambda>(\<D>, \<V>, \<V>'). do {
-    (mem, k) \<leftarrow> SPEC(\<lambda>(mem, k::'nat). \<not>alloc_failed mem \<longrightarrow> k \<notin># dom_m \<V>);
-    if alloc_failed mem then do {k \<leftarrow> RES (UNIV :: 'nat set); RETURN (mem, (\<D>, \<V>, \<V>'), k)}
-    else RETURN (Allocated, (add_mset v \<D>, fmupd k v \<V>, fmupd v k \<V>'), k)
-  })\<close>
-
-definition import_variable
-  :: \<open>'string \<Rightarrow> ('nat, 'string) vars \<Rightarrow> (memory_allocation \<times> ('nat, 'string) vars \<times> 'string) nres\<close>
-  where
-  \<open>import_variable v = (\<lambda>\<V>. do {
-     ASSERT(v \<notin># \<V>);
-     SPEC(\<lambda>(mem, \<V>', k::'string). \<not>alloc_failed mem \<longrightarrow> \<V>' = add_mset k \<V> \<and> k = v)
-  })\<close>
-
-definition is_new_variableS :: \<open>'string \<Rightarrow> ('nat, 'string) shared_vars \<Rightarrow> bool nres\<close> where
-  \<open>is_new_variableS v = (\<lambda>(\<D>, \<V>, \<V>').
+definition is_new_variable_c :: \<open>'string \<Rightarrow> ('string, 'nat) shared_vars_c \<Rightarrow> bool nres\<close> where
+  \<open>is_new_variable_c v = (\<lambda>(\<V>, \<V>').
   RETURN (v \<notin># dom_m \<V>')
   )\<close>
 
-definition is_new_variable :: \<open>'string \<Rightarrow> ('nat, 'string) vars \<Rightarrow> bool nres\<close> where
-  \<open>is_new_variable v = (\<lambda>\<V>'.
-    RETURN (v \<notin># \<V>')
-  )\<close>
+lemma fset_fmdom_dom_m: \<open>fset (fmdom A) = set_mset (dom_m A)\<close>
+  by (simp add: dom_m_def)
 
-lemma import_variableS_import_variable:
-  fixes \<V> :: \<open>('nat, 'string) vars\<close>
-  assumes \<open>(\<A>, \<V>) \<in> perfectly_shared_vars_rel\<close> and \<open>(v, v') \<in> Id\<close>
-  shows \<open>import_variableS v \<A> \<le> \<Down>({((mem, \<A>', i), (mem', \<V>', j)). mem = mem' \<and>
-      (\<A>', \<V>') \<in> perfectly_shared_vars_rel \<and>
-      (\<not>alloc_failed mem' \<longrightarrow> (i, j) \<in> perfectly_shared_var_rel \<A>') \<and>
-      (\<forall>xs. xs \<in> perfectly_shared_var_rel \<A> \<longrightarrow> xs \<in> perfectly_shared_var_rel \<A>')})
-    (import_variable v' \<V>)\<close>
-  using assms
-  unfolding import_variableS_def import_variable_def
-  by (refine_vcg lhs_step_If)
-   (auto intro!: RETURN_RES_refine simp:  perfectly_shared_add_new_var perfectly_shared_vars_rel_def
-    perfectly_shared_var_rel_def br_def)
-
-lemma is_new_variable_spec:
-  assumes \<open>(\<A>, \<D>\<V>) \<in> perfectly_shared_vars_rel\<close> \<open>(v,v') \<in> Id\<close>
-  shows \<open>is_new_variableS v \<A> \<le> \<Down>bool_rel (is_new_variable v' \<D>\<V>)\<close>
-  using assms
-  unfolding is_new_variable_def is_new_variableS_def
-  by (auto simp: perfectly_shared_vars_rel_def
-    perfectly_shared_vars_simps split: prod.splits)
+lemma fmap_rel_nat_rel_dom_m_iff:
+  \<open>(A, B) \<in> \<langle>R, S\<rangle>fmap_rel \<Longrightarrow> (v,v')\<in>R \<Longrightarrow> v\<in>#dom_m A \<longleftrightarrow>v'\<in># dom_m B\<close>
+  by (auto simp: fmap_rel_alt_def distinct_mset_dom fset_fmdom_dom_m
+    dest!: multi_member_split
+    simp del: fmap_rel_nat_the_fmlookup)
 
 
-definition get_var_name :: \<open>('nat, 'string) vars \<Rightarrow> 'string \<Rightarrow>  'string nres\<close> where
-  \<open>get_var_name \<V> x = do {
-    ASSERT(x \<in># \<V>);
-    RETURN x
-  }\<close>
-definition get_var_nameS :: \<open>('nat, 'string) shared_vars \<Rightarrow> 'string \<Rightarrow> 'nat nres\<close> where
-  \<open>get_var_nameS \<V> x = do {
-    ASSERT(x \<in># dom_m (snd (snd \<V>)));
-    RETURN (snd (snd \<V>) \<propto> x)
-  }\<close>
+lemma is_new_variable_c_is_new_variableS:
+  shows \<open>(uncurry is_new_variable_c, uncurry is_new_variableS) \<in> R \<times>\<^sub>r perfect_shared_vars_rel_c R \<rightarrow>\<^sub>f \<langle>bool_rel\<rangle>nres_rel\<close>
+  by (use  in \<open>auto simp: perfect_shared_vars_rel_c_def fmap_rel_nat_rel_dom_m
+    fmap_rel_nat_rel_dom_m_iff is_new_variable_c_def is_new_variableS_def
+    intro!: frefI nres_relI\<close>)
 
-lemma get_var_nameS_spec:
-  fixes \<D>\<V> :: \<open>('nat, 'string) vars\<close> and
-    \<A> :: \<open>('nat, 'string) shared_vars\<close> and
-    x :: 'string
-  assumes \<open>(\<A>, \<D>\<V>) \<in> perfectly_shared_vars_rel\<close> and
-    \<open>(x,x') \<in> Id\<close>
-  shows \<open>get_var_nameS \<A> x \<le> \<Down>(perfectly_shared_var_rel \<A>) (get_var_name \<D>\<V> x')\<close>
-  using assms unfolding get_var_nameS_def get_var_name_def
+
+definition get_var_pos_c :: \<open> ('string, nat) shared_vars_c \<Rightarrow> _ \<Rightarrow> nat nres\<close> where
+  \<open>get_var_pos_c = (\<lambda>(xs, \<V>) x. do {
+    ASSERT(x \<in># dom_m \<V>);
+    RETURN (the (fmlookup \<V> x))
+  })\<close>
+
+
+lemma get_var_pos_c_get_var_posS:
+  fixes A' :: \<open>(nat,'string) shared_vars\<close>
+  assumes
+    V: \<open>single_valued R\<close> \<open>single_valued (R\<inverse>)\<close>
+  shows \<open>(uncurry get_var_pos_c, uncurry get_var_posS) \<in> perfect_shared_vars_rel_c R \<times>\<^sub>r R \<rightarrow>\<^sub>f \<langle>nat_rel\<rangle>nres_rel\<close>
+  unfolding get_var_pos_c_def get_var_posS_def uncurry_def
+    apply (clarify intro!: frefI nres_relI)
   apply refine_vcg
-  apply (auto simp: perfectly_shared_var_rel_def
-    perfectly_shared_vars_rel_def perfectly_shared_vars_simps br_def
-    intro!: ASSERT_leI)
-  apply (simp_all add: perfectly_shared_vars_def in_dom_m_lookup_iff)
-  done
-
-abbreviation perfectly_shared_monom
-  :: \<open>('nat,'string) shared_vars \<Rightarrow> ('nat list \<times> 'string list) set\<close>
-where
-  \<open>perfectly_shared_monom \<V> \<equiv> \<langle>perfectly_shared_var_rel \<V>\<rangle>list_rel \<close>
-
-definition import_monom_no_newS
-  :: \<open>('nat, 'string) shared_vars \<Rightarrow> 'string list \<Rightarrow> (bool \<times> 'nat list) nres\<close>
-where
-  \<open>import_monom_no_newS \<A> xs = do {
-  (new, _, xs) \<leftarrow> WHILE\<^sub>T (\<lambda>(new, xs, _). \<not>new \<and> xs \<noteq> [])
-    (\<lambda>(_, xs, ys). do {
-      ASSERT(xs \<noteq> []);
-      let x = hd xs;
-      b \<leftarrow> is_new_variableS x \<A>;
-      if b
-      then RETURN (True, tl xs, ys)
-      else do {
-        x \<leftarrow> get_var_nameS \<A> x;
-        RETURN (False, tl xs, ys @ [x])
-       }
-    })
-    (False, xs, []);
-  RETURN (new, xs)
- }\<close>
-
-definition import_monom_no_new
-  :: \<open>('nat, 'string) vars \<Rightarrow> 'string list \<Rightarrow> (bool \<times> 'string list) nres\<close>
-where
-  \<open>import_monom_no_new \<A> xs = do {
-  (new, _, xs) \<leftarrow> WHILE\<^sub>T (\<lambda>(new, xs, _). \<not>new \<and> xs \<noteq> [])
-  (\<lambda>(_, xs, ys). do {
-    ASSERT(xs \<noteq> []);
-    let x = hd xs;
-    b \<leftarrow> is_new_variable x \<A>;
-    if b
-    then RETURN (True, tl xs, ys)
-      else do {
-      x \<leftarrow> get_var_name \<A> x;
-      RETURN (False, tl xs, ys @ [x])
-    }
-    })
-    (False, xs, []);
-  RETURN (new, xs)
-}\<close>
-
-lemma import_monom_no_new_spec:
-  shows \<open>import_monom_no_new \<A> xs \<le> \<Down> Id
-    (SPEC(\<lambda>(new, ys). (new \<longleftrightarrow> \<not>set xs \<subseteq> set_mset \<A>) \<and>
-      (\<not>new \<longrightarrow> ys = xs)))\<close>
-  unfolding import_monom_no_new_def is_new_variable_def get_var_name_def
-  apply (refine_vcg
-    WHILET_rule[where I = \<open>(\<lambda>(new, ys, zs). (\<not>new \<longrightarrow> xs = zs @ ys) \<and> (\<not>new \<longrightarrow> set zs \<subseteq> set_mset \<A>) \<and>
-     (new \<longrightarrow> \<not>set xs \<subseteq> set_mset \<A>))\<close> and
-    R = \<open>measure (\<lambda>(_, ys, _). length ys)\<close>])
-  subgoal by auto
-  subgoal by auto
-  subgoal by auto
-  subgoal by auto
-  subgoal by auto
-  subgoal by auto
-  subgoal by (auto simp: neq_Nil_conv)
-  subgoal by (auto simp: neq_Nil_conv)
-  subgoal by auto
-  subgoal by auto
-  subgoal by auto
-  subgoal by auto
-  subgoal by auto
-  subgoal by auto
-  subgoal by auto
-  subgoal by auto
-  done
-
-lemma import_monom_no_newS_import_monom_no_new:
-  assumes \<open>(\<A>, \<V>\<D>) \<in> perfectly_shared_vars_rel\<close> \<open>(xs, xs') \<in> Id\<close>
-  shows \<open>import_monom_no_newS \<A> xs \<le> \<Down>(bool_rel \<times>\<^sub>r perfectly_shared_monom \<A>)
-    (import_monom_no_new \<V>\<D> xs')\<close>
-  using assms
-  unfolding import_monom_no_new_def import_monom_no_newS_def
-  apply (refine_rcg WHILET_refine[where R = \<open>bool_rel \<times>\<^sub>r \<langle>Id\<rangle>list_rel \<times>\<^sub>r perfectly_shared_monom \<A>\<close>]
-    is_new_variable_spec get_var_nameS_spec)
-  subgoal by auto
+  subgoal using assms by (auto simp: perfect_shared_vars_rel_c_def fmap_rel_nat_rel_dom_m_iff)
   subgoal
-    by auto
-  subgoal
-    by auto 
-  subgoal by auto
-  subgoal by auto
-  subgoal by auto
-  subgoal by auto
-  subgoal by (force simp: list_rel_append1)
-  subgoal by auto
+    using assms by (auto simp: perfect_shared_vars_rel_c_def fmap_rel_nat_rel_dom_m_iff dest: fmap_rel_fmlookup_rel)
   done
 
- definition import_poly_no_newS
-  :: \<open>('nat, 'string) shared_vars \<Rightarrow> ('string list \<times> 'a) list \<Rightarrow> (bool \<times> ('nat list \<times> 'a)list) nres\<close>
-where
-  \<open>import_poly_no_newS \<A> xs = do {
-  (new, _, xs) \<leftarrow> WHILE\<^sub>T (\<lambda>(new, xs, _). \<not>new \<and> xs \<noteq> [])
-    (\<lambda>(_, xs, ys). do {
-      ASSERT(xs \<noteq> []);
-      let (x, n) = hd xs;
-      (b, x) \<leftarrow> import_monom_no_newS \<A> x;
-      if b
-      then RETURN (True, tl xs, ys)
-      else do {
-        RETURN (False, tl xs, ys @ [(x, n)])
-       }
-    })
-    (False, xs, []);
-  RETURN (new, xs)
- }\<close>
+abbreviation perfect_shared_vars_assn :: \<open>(string, nat) shared_vars_c \<Rightarrow> _ \<Rightarrow> assn\<close> where
+  \<open>perfect_shared_vars_assn \<equiv> arl_assn string_assn \<times>\<^sub>a hm_fmap_assn string_assn uint64_nat_assn\<close>
+abbreviation shared_vars_assn where
+  \<open>shared_vars_assn \<equiv> hr_comp perfect_shared_vars_assn (perfect_shared_vars_rel_c Id)\<close>
 
-definition import_poly_no_new
-  :: \<open>('nat, 'string) vars \<Rightarrow> ('string list \<times> 'a) list \<Rightarrow> (bool \<times> ('string list \<times> 'a) list) nres\<close>
-where
-  \<open>import_poly_no_new \<A> xs = do {
-  (new, _, xs) \<leftarrow> WHILE\<^sub>T (\<lambda>(new, xs, _). \<not>new \<and> xs \<noteq> [])
-  (\<lambda>(_, xs, ys). do {
-    ASSERT(xs \<noteq> []);
-    let (x, n) = hd xs;
-    (b, x) \<leftarrow> import_monom_no_new \<A> x;
-    if b
-    then RETURN (True, tl xs, ys)
-      else do {
-      RETURN (False, tl xs, ys @ [(x, n)])
-    }
-    })
-    (False, xs, []);
-  RETURN (new, xs)
-}\<close>
+lemmas [sepref_fr_rules] = hm.lookup_hnr[FCOMP op_map_lookup_fmlookup]
 
+sepref_definition get_var_pos_c_impl
+  is \<open>uncurry get_var_pos_c\<close>
+  :: \<open>perfect_shared_vars_assn\<^sup>k *\<^sub>a string_assn\<^sup>k \<rightarrow>\<^sub>a uint64_nat_assn\<close>
+  supply [simp] = in_dom_m_lookup_iff
+  unfolding get_var_pos_c_def fmlookup'_def[symmetric]
+  by sepref
 
-lemma import_poly_no_newS_import_poly_no_new:
-  assumes \<open>(\<A>, \<V>\<D>) \<in> perfectly_shared_vars_rel\<close> \<open>(xs, xs') \<in> Id\<close>
-  shows \<open>import_poly_no_newS \<A> xs \<le> \<Down>(bool_rel \<times>\<^sub>r \<langle>perfectly_shared_monom \<A> \<times>\<^sub>r Id\<rangle>list_rel)
-    (import_poly_no_new \<V>\<D> xs')\<close>
-  using assms
-  unfolding import_poly_no_new_def import_poly_no_newS_def
-  apply (refine_rcg WHILET_refine[where
-    R = \<open>bool_rel \<times>\<^sub>r \<langle>Id\<rangle>list_rel \<times>\<^sub>r \<langle>perfectly_shared_monom \<A> \<times>\<^sub>r Id\<rangle>list_rel\<close>]
-    import_monom_no_newS_import_monom_no_new)
-  subgoal by auto
-  subgoal by auto
-  subgoal by auto
-  subgoal by auto
-  subgoal by auto
-  subgoal by auto
-  subgoal by (force simp: list_rel_append1)
-  subgoal by auto
-  done
+sepref_definition is_new_variable_c_impl
+  is \<open>uncurry is_new_variable_c\<close>
+  :: \<open>string_assn\<^sup>k  *\<^sub>a  perfect_shared_vars_assn\<^sup>k \<rightarrow>\<^sub>a bool_assn\<close>
+  supply [simp] = in_dom_m_lookup_iff
+  unfolding is_new_variable_c_def fmlookup'_def[symmetric] in_dom_m_lookup_iff
+  by sepref
 
-lemma import_poly_no_new_spec:
-  shows \<open>import_poly_no_new \<A> xs \<le> \<Down> Id
-    (SPEC(\<lambda>(new, ys). \<not>new \<longrightarrow> ys = xs \<and> vars_llist xs \<subseteq> set_mset \<A>))\<close>
-proof -
-  define I where
-    [simp]: \<open>I = (\<lambda>(new, ys, zs). \<not>new \<longrightarrow> (xs = zs @ ys \<and> vars_llist zs \<subseteq> set_mset \<A>))\<close>
-  show ?thesis
-  unfolding import_poly_no_new_def is_new_variable_def get_var_name_def import_variable_def
-  apply (refine_vcg import_monom_no_new_spec[THEN order_trans]
-    WHILET_rule[where I = \<open>I\<close> and
-    R = \<open>measure (\<lambda>(mem, ys, _). (if mem then 0 else 1) + length ys)\<close>])
-  subgoal by auto
-  subgoal by auto
-  subgoal by auto
-  subgoal by (auto simp: neq_Nil_conv)
-  subgoal by auto
-  subgoal by auto
-  done
-qed
+lemma [sepref_fr_rules]:
+  \<open>(uncurry is_new_variable_c_impl, uncurry is_new_variableS) \<in> string_assn\<^sup>k *\<^sub>a shared_vars_assn\<^sup>k \<rightarrow>\<^sub>a bool_assn\<close>
+  using is_new_variable_c_impl.refine[FCOMP is_new_variable_c_is_new_variableS, of Id]
+  by auto
 
-definition import_monomS
-  :: \<open>('nat, 'string) shared_vars \<Rightarrow> 'string list \<Rightarrow> (_ \<times> 'nat list \<times> ('nat, 'string) shared_vars) nres\<close>
-where
-  \<open>import_monomS \<A> xs = do {
-  (new, _, xs, \<A>) \<leftarrow> WHILE\<^sub>T (\<lambda>(mem, xs, _, _). \<not>alloc_failed mem \<and> xs \<noteq> [])
-    (\<lambda>(_, xs, ys, \<A>). do {
-      ASSERT(xs \<noteq> []);
-      let x = hd xs;
-      b \<leftarrow> is_new_variableS x \<A>;
-      if b
-      then do {
-        (mem, \<A>, x) \<leftarrow> import_variableS x \<A>;
-        if alloc_failed mem
-        then RETURN (mem, xs, ys, \<A>)
-        else RETURN (mem, tl xs, ys @ [x], \<A>)
-      }
-      else do {
-        x \<leftarrow> get_var_nameS \<A> x;
-        RETURN (Allocated, tl xs, ys @ [x], \<A>)
-       }
-    })
-    (Allocated, xs, [], \<A>);
-  RETURN (new, xs, \<A>)
- }\<close>
+lemma [sepref_fr_rules]:
+  \<open>(uncurry get_var_pos_c_impl, uncurry get_var_posS) \<in> shared_vars_assn\<^sup>k *\<^sub>a string_assn\<^sup>k \<rightarrow>\<^sub>a uint64_nat_assn\<close>
+  using get_var_pos_c_impl.refine[FCOMP get_var_pos_c_get_var_posS, of Id]
+  by auto
 
-definition import_monom
-  :: \<open>('nat, 'string) vars \<Rightarrow> 'string list \<Rightarrow> (memory_allocation \<times> 'string list \<times> ('nat, 'string) vars) nres\<close>
-where
-  \<open>import_monom \<A> xs = do {
-  (new, _, xs, \<A>) \<leftarrow> WHILE\<^sub>T (\<lambda>(new, xs, _, _). \<not>alloc_failed new \<and> xs \<noteq> [])
-  (\<lambda>(mem, xs, ys, \<A>). do {
-  ASSERT(xs \<noteq> []);
-  let x = hd xs;
-    b \<leftarrow> is_new_variable x \<A>;
-    if b
-  then do {
-    (mem, \<A>, x) \<leftarrow> import_variable x \<A>;
-    if alloc_failed mem
-    then RETURN (mem, xs, ys, \<A>)
-    else RETURN (mem, tl xs, ys @ [x], \<A>)
-    }
-    else do {
-    x \<leftarrow> get_var_name \<A> x;
-    RETURN (mem, tl xs, ys @ [x], \<A>)
-    }
-    })
-    (Allocated, xs, [], \<A>);
-    RETURN (new, xs, \<A>)
-    }\<close>
-
-lemma import_monom_spec:
-  shows \<open>import_monom \<A> xs \<le> \<Down> Id
-    (SPEC(\<lambda>(new, ys, \<A>'). \<not>alloc_failed new \<longrightarrow> ys = xs \<and> set_mset \<A>' = set_mset \<A> \<union> set xs))\<close>
-proof -
-  define I where
-    [simp]: \<open>I = (\<lambda>(new, ys, zs, \<A>'). \<not>alloc_failed new \<longrightarrow> (xs = zs @ ys \<and> set_mset \<A>' = set_mset \<A> \<union> set zs))\<close>
-  show ?thesis
-  unfolding import_monom_def is_new_variable_def get_var_name_def import_variable_def
-  apply (refine_vcg
-    WHILET_rule[where I = \<open>I\<close> and
-    R = \<open>measure (\<lambda>(mem, ys, _). (if alloc_failed mem then 0 else 1) + length ys)\<close>])
-  subgoal by auto
-  subgoal by auto
-  subgoal by auto
-  subgoal by (auto simp: neq_Nil_conv)
-  subgoal by auto
-  subgoal by auto
-  subgoal by auto
-  subgoal by auto
-  subgoal by auto
-  subgoal by auto
-  subgoal by auto
-  subgoal by auto
-  done
-qed
-
-definition import_polyS
-  :: \<open>('nat, 'string) shared_vars \<Rightarrow> ('string list \<times> 'a) list \<Rightarrow> 
-    (memory_allocation \<times> ('nat list \<times> 'a)list \<times> ('nat, 'string) shared_vars) nres\<close>
-  where
-  \<open>import_polyS \<A> xs = do {
-  (mem,_, xs, \<A>) \<leftarrow> WHILE\<^sub>T (\<lambda>(mem, xs, _, _). \<not>alloc_failed mem \<and> xs \<noteq> [])
-    (\<lambda>(mem, xs, ys, \<A>). do {
-      ASSERT(xs \<noteq> []);
-      let (x, n) = hd xs;
-      (mem, x, \<A>) \<leftarrow> import_monomS \<A> x;
-      if alloc_failed mem
-      then RETURN (mem, xs, ys, \<A>)
-      else do {
-       RETURN (mem, tl xs, ys @ [(x, n)], \<A>)
-      }
-    }) 
-    (Allocated, xs, [], \<A>);
-   RETURN (mem, xs, \<A>)
- }\<close>
-
-definition import_poly
-  :: \<open>('nat, 'string) vars \<Rightarrow> ('string list \<times> 'a) list \<Rightarrow>
-        (memory_allocation \<times> ('string list \<times> 'a) list \<times> ('nat, 'string)vars) nres\<close>
-  where
-  \<open>import_poly \<A> xs = do {
-  (new, _, xs, \<A>) \<leftarrow> WHILE\<^sub>T (\<lambda>(new, xs, _). \<not>alloc_failed new \<and> xs \<noteq> [])
-  (\<lambda>(_, xs, ys, \<A>). do {
-    ASSERT(xs \<noteq> []);
-    let (x, n) = hd xs;
-    (b, x, \<A>) \<leftarrow> import_monom \<A> x;
-    if alloc_failed b
-    then RETURN (b, xs, ys, \<A>)
-    else do {
-      RETURN (Allocated, tl xs, ys @ [(x, n)], \<A>)
-    }
-  })
-  (Allocated, xs, [], \<A>);
-  RETURN (new, xs, \<A>)
-}\<close>
-
-lemma import_poly_spec:
-  fixes \<A> :: \<open>('nat, 'string) vars\<close>
-  shows \<open>import_poly \<A> xs \<le> \<Down> Id
-    (SPEC(\<lambda>(new, ys, \<A>'). \<not>alloc_failed new \<longrightarrow> ys = xs \<and> set_mset \<A>' = set_mset \<A> \<union> \<Union>(set `fst ` set xs)))\<close>
-proof -
-  define I where
-    [simp]: \<open>I = (\<lambda>(new, ys, zs, \<A>'). \<not>alloc_failed new \<longrightarrow> (xs = zs @ ys \<and>
-       set_mset \<A>' = set_mset \<A> \<union> \<Union>(set ` fst ` set zs)))\<close>
-  show ?thesis
-    unfolding import_poly_def is_new_variable_def get_var_name_def import_variable_def
-    apply (refine_vcg import_monom_spec[THEN order_trans]
-      WHILET_rule[where I = \<open>I\<close> and
-      R = \<open>measure (\<lambda>(mem, ys, _). (if alloc_failed mem then 0 else 1) + length ys)\<close>])
-    subgoal by auto
-    subgoal by auto
-    subgoal by auto
-    subgoal by (auto simp: neq_Nil_conv)
-    subgoal by auto
-    subgoal by auto
-    done
-qed
-
-lemma list_rel_append_single: \<open>(xs, ys) \<in> \<langle>R\<rangle>list_rel \<Longrightarrow> (x, y) \<in> R \<Longrightarrow> (xs @ [x], ys @ [y]) \<in> \<langle>R\<rangle>list_rel\<close>
-  by (meson list_rel_append1 list_rel_simp(4) refine_list(1))
-
-lemma list_rel_mono: \<open>A \<in> \<langle>R\<rangle>list_rel \<Longrightarrow> (\<And>xs. xs \<in> R \<Longrightarrow> xs \<in> R') \<Longrightarrow> A \<in> \<langle>R'\<rangle>list_rel\<close>
-  unfolding list_rel_def
-  apply (cases A)
-  by (simp add: list_all2_mono)
-
-lemma import_monomS_import_monom:
-  fixes \<V>\<D> :: \<open>('nat, 'string) vars\<close> and \<A>\<^sub>0 :: \<open>('nat, 'string)shared_vars\<close> and xs xs' :: \<open>'string list\<close>
-  assumes \<open>(\<A>\<^sub>0, \<V>\<D>) \<in> perfectly_shared_vars_rel\<close> \<open>(xs, xs') \<in> \<langle>Id\<rangle>list_rel\<close>
-  shows \<open>import_monomS \<A>\<^sub>0 xs \<le> \<Down> {((mem, xs\<^sub>0, \<A>), (mem', ys\<^sub>0, \<A>')). mem = mem' \<and> 
-    (\<A>, \<A>') \<in> perfectly_shared_vars_rel \<and>  (\<not>alloc_failed mem \<longrightarrow> (xs\<^sub>0, ys\<^sub>0) \<in> perfectly_shared_monom \<A>)\<and>
-    (\<not>alloc_failed mem \<longrightarrow> (\<forall>xs. xs \<in> perfectly_shared_monom \<A>\<^sub>0 \<longrightarrow> xs \<in> perfectly_shared_monom \<A>))}
-    (import_monom \<V>\<D> xs')\<close>
-  using assms
-  unfolding import_monom_def import_monomS_def
-  apply (refine_rcg WHILET_refine[where
-    R = \<open>{((mem::memory_allocation, xs\<^sub>0::'string list, zs\<^sub>0::'nat list,  \<A> :: ('nat, 'string)shared_vars),
-    (mem', ys\<^sub>0::'string list, zs\<^sub>0'::'string list, \<A>' :: ('nat, 'string)vars)). mem = mem' \<and>
-    (\<A>, \<A>') \<in> perfectly_shared_vars_rel \<and> (\<not>alloc_failed mem \<longrightarrow> (zs\<^sub>0, zs\<^sub>0') \<in> perfectly_shared_monom \<A>) \<and>
-    (xs\<^sub>0, ys\<^sub>0) \<in> \<langle>Id\<rangle>list_rel \<and>
-    (\<not>alloc_failed mem \<longrightarrow> (\<forall>xs. xs \<in> perfectly_shared_monom \<A>\<^sub>0 \<longrightarrow> xs \<in> perfectly_shared_monom \<A>))}\<close>]
-    import_variableS_import_variable
-    is_new_variable_spec get_var_nameS_spec)
-  subgoal by auto
-  subgoal
-    by auto
-  subgoal
-    by auto 
-  subgoal by auto
-  subgoal by auto
-  subgoal by auto
-  subgoal by auto
-  subgoal by auto
-  subgoal by auto
-  subgoal by auto
-  subgoal apply (auto intro!: list_rel_append_single intro: list_rel_mono)
-    by (metis (full_types) EPAC_Perfectly_Shared_Vars.list_rel_mono surj_pair)
-  subgoal by auto
-  subgoal by auto
-  subgoal using memory_allocation.exhaust_disc  by (auto intro!: list_rel_append_single intro: list_rel_mono)
-  subgoal by auto
-  done
-
-lemma import_polyS_import_poly:
-  assumes \<open>(\<A>, \<V>\<D>) \<in> perfectly_shared_vars_rel\<close> \<open>(xs, xs') \<in>  \<langle>\<langle>Id\<rangle>list_rel\<times>\<^sub>rId\<rangle>list_rel\<close>
-  shows \<open>import_polyS \<A> xs \<le> \<Down> {((mem, xs\<^sub>0, \<A>), (mem', ys\<^sub>0, \<A>')). mem = mem' \<and> 
-    (\<A>, \<A>') \<in> perfectly_shared_vars_rel \<and>  (\<not>alloc_failed mem \<longrightarrow> (xs\<^sub>0, ys\<^sub>0) \<in> \<langle>perfectly_shared_monom \<A> \<times>\<^sub>r Id\<rangle>list_rel)}
-    (import_poly \<V>\<D> xs')\<close>
-  using assms
-  unfolding import_poly_def import_polyS_def
-  apply (refine_rcg WHILET_refine[where
-    R = \<open>{((mem, zs, xs\<^sub>0, \<A>), (mem', zs', ys\<^sub>0, \<A>')). mem = mem' \<and> 
-    (\<A>, \<A>') \<in> perfectly_shared_vars_rel \<and> (zs, zs') \<in> \<langle>\<langle>Id\<rangle>list_rel \<times>\<^sub>r Id\<rangle>list_rel
-    \<and> (\<not>alloc_failed mem \<longrightarrow> (xs\<^sub>0, ys\<^sub>0) \<in> \<langle>perfectly_shared_monom \<A> \<times>\<^sub>r Id\<rangle>list_rel)}\<close>]
-    import_monomS_import_monom)
-  subgoal by auto
-  subgoal by auto
-  subgoal by auto
-  subgoal by auto
-  subgoal by auto
-  subgoal by auto
-  subgoal by (force simp: list_rel_append1)
-  subgoal for x x' x1 x2 x1a x2a x1b x2b x1c x2c x1d x2d x1e x2e x1f x2f x1g x2g xa x'a x1h x2h x1i x2i
-    x1j x2j x1k x2k
-    using memory_allocation.exhaust_disc[of x1h \<open>x1h = Allocated\<close>]
-    by (auto intro!: list_rel_append_single intro: list_rel_mono)
-  subgoal by auto
-    done
-
-
-
-definition drop_content :: \<open>'string \<Rightarrow> ('nat, 'string) vars \<Rightarrow> ('nat, 'string) vars nres\<close>
-  where
-  \<open>drop_content = (\<lambda>v \<V>'. do {
-    ASSERT(v \<in># \<V>');
-    RETURN (remove1_mset v \<V>')
-  })\<close>
-
-
-definition drop_contentS :: \<open>'string \<Rightarrow> ('nat, 'string) shared_vars \<Rightarrow> ('nat, 'string) shared_vars nres\<close>
-  where
-  \<open>drop_contentS = (\<lambda>v (\<D>, \<V>, \<V>'). do {
-    ASSERT(v \<in># dom_m \<V>');
-    if count \<D> v = 1
-    then do {
-      let i = \<V>' \<propto> v;
-      RETURN (remove1_mset v \<D>, fmdrop i \<V>, fmdrop v \<V>')
-    }
-    else
-    RETURN (remove1_mset v \<D>, \<V>, \<V>')
-  })\<close>
-
-lemma drop_contentS_drop_content:
-  assumes \<open>(\<A>, \<V>\<D>) \<in> perfectly_shared_vars_rel\<close> \<open>(v, v') \<in> Id\<close> 
-  shows \<open>drop_contentS v \<A> \<le> \<Down>perfectly_shared_vars_rel (drop_content v' \<V>\<D>)\<close>
-proof -
-  have [simp]: \<open>count xs x = 1 \<Longrightarrow> y \<in># remove1_mset x xs \<longleftrightarrow> y \<in># xs \<and> x \<noteq>y\<close> for x xs y
-    by (auto simp add: in_diff_count)
-  have [simp]: \<open>count xs x \<noteq> 1 \<Longrightarrow> x \<in># xs \<Longrightarrow> y \<in># remove1_mset x xs \<longleftrightarrow> y \<in># xs\<close> for x xs y
-    by (metis One_nat_def add_mset_remove_trivial_eq count_add_mset count_inI in_remove1_mset_neq)
-  show ?thesis
-    using assms
-    unfolding drop_content_def drop_contentS_def
-    apply refine_vcg
-    apply (auto simp: perfectly_shared_vars_rel_def perfectly_shared_vars_def
-      distinct_mset_dom distinct_mset_remove1_All)
-    by (metis option.inject)
-qed
-
-definition perfectly_shared_strings_equal
-  :: \<open>('nat, 'string) vars \<Rightarrow> 'string \<Rightarrow> 'string \<Rightarrow> bool nres\<close>
-where
-  \<open>perfectly_shared_strings_equal \<V> x y = do {
-    ASSERT(x \<in># \<V> \<and> y \<in># \<V>);
-    RETURN (x = y)
-  }\<close>
-
-definition perfectly_shared_strings_equal_l
-  :: \<open>('nat,'string)shared_vars \<Rightarrow> 'nat \<Rightarrow> 'nat \<Rightarrow> bool nres\<close>
-where
-  \<open>perfectly_shared_strings_equal_l \<V> x y = do {
-    RETURN (x = y)
-  }\<close>
-
-lemma perfectly_shared_strings_equal_l_perfectly_shared_strings_equal:
-  assumes \<open>(\<A>, \<V>) \<in> perfectly_shared_vars_rel\<close> and
-    \<open>(x, x') \<in> perfectly_shared_var_rel \<A>\<close> and
-    \<open>(y, y') \<in> perfectly_shared_var_rel \<A>\<close>
-  shows \<open>perfectly_shared_strings_equal_l \<A> x y \<le> \<Down>bool_rel (perfectly_shared_strings_equal \<V> x' y')\<close>
-  using assms unfolding perfectly_shared_strings_equal_l_def perfectly_shared_strings_equal_def
-    perfectly_shared_vars_rel_def perfectly_shared_var_rel_def br_def
-  by refine_rcg
-    (auto simp: perfectly_shared_vars_def simp: add_mset_eq_add_mset dest!: multi_member_split)
+    term perfect_shared_term_order_rel
 
 end
